computation/computation_lib_extends.v
@@ -1,0 +1,665 @@
+(*
+
+  Copyright 2014 Cornell University
+  Copyright 2015 Cornell University
+  Copyright 2016 Cornell University
+  Copyright 2017 Cornell University
+
+  This file is part of VPrl (the Verified Nuprl project).
+
+  VPrl is free software: you can redistribute it and/or modify
+  it under the terms of the GNU General Public License as published by
+  the Free Software Foundation, either version 3 of the License, or
+  (at your option) any later version.
+
+  VPrl is distributed in the hope that it will be useful,
+  but WITHOUT ANY WARRANTY; without even the implied warranty of
+  MERCHANTABILITY or FITNESS FOR A PARTICULAR PURPOSE.  See the
+  GNU General Public License for more details.
+
+  You should have received a copy of the GNU General Public License
+  along with VPrl.  If not, see <http://www.gnu.org/licenses/>.
+
+
+  Websites: http://nuprl.org/html/verification/
+            http://nuprl.org/html/Nuprl2Coq
+            https://github.com/vrahli/NuprlInCoq
+
+  Authors: Vincent Rahli
+
+ *)
+
+
+Require Export computation_preserves_lib.
+
+
+Definition opabs_of_lib_entry {o} (e : @library_entry o) : opabs :=
+  match e with
+  | lib_abs oa _ _ _ => oa
+  end.
+
+Definition matching_entries {o} (entry1 entry2 : @library_entry o) : Prop :=
+  matching_entry_sign (opabs_of_lib_entry entry1) (opabs_of_lib_entry entry2).
+
+Fixpoint entry_in_library {o} (entry : @library_entry o) (lib : library) : Type :=
+  match lib with
+  | [] => False
+  | entry' :: entries =>
+    entry = entry'
+    [+]
+    (~ matching_entries entry entry'
+       # entry_in_library entry entries)
+  end.
+
+(* [lib1] extends [lib0] *)
+Definition lib_extends {o} (lib1 lib0 : @library o) : Type :=
+  forall entry, entry_in_library entry lib0 -> entry_in_library entry lib1.
+
+Definition in_lib {o}
+           (opabs : opabs)
+           (lib   : @library o) :=
+  {e : library_entry
+   & LIn e lib
+   # matching_entry_sign opabs (opabs_of_lib_entry e)}.
+
+Definition entry_not_in_lib {o} (e : @library_entry o) (l : @library o) :=
+  !in_lib (opabs_of_lib_entry e) l.
+
+Hint Resolve matching_entry_sign_sym : slow.
+
+Lemma entry_in_library_implies_in {o} :
+  forall (entry : @library_entry o) lib,
+    entry_in_library entry lib -> LIn entry lib.
+Proof.
+  induction lib; auto; introv h; simpl in *.
+  repndors; subst; tcsp.
+Qed.
+Hint Resolve entry_in_library_implies_in : slow.
+
+Lemma lib_extends_cons_implies {o} :
+  forall (e : @library_entry o) (lib lib0 : library),
+    entry_not_in_lib e lib0
+    -> lib_extends lib (e :: lib0)
+    -> lib_extends lib lib0.
+Proof.
+  introv ni ext i.
+  apply ext; simpl; clear ext.
+  right; dands; auto; intro m.
+  destruct ni.
+
+  exists entry.
+  dands; eauto 3 with slow.
+Qed.
+
+Lemma lib_extends_refl {o} :
+  forall (lib : @library o), lib_extends lib lib.
+Proof.
+  introv i; auto.
+Qed.
+Hint Resolve lib_extends_refl : slow.
+
+Lemma entry_in_library_implies_find_entry {o} :
+  forall (lib : @library o) abs opabs vars bs rhs correct,
+    matching_entry abs opabs vars bs
+    -> entry_in_library (lib_abs opabs vars rhs correct) lib
+    -> find_entry lib abs bs = Some (lib_abs opabs vars rhs correct).
+Proof.
+  induction lib; introv m e; simpl in *; tcsp.
+  destruct a.
+  repndors; repnd.
+
+  - inversion e; subst; clear e.
+    boolvar; tcsp.
+
+    + pose proof (correct_abs_proof_irrelevance _ _ _ correct correct0) as xx; subst; auto.
+
+    + apply not_matching_entry_iff in n; tcsp.
+
+  - boolvar; tcsp.
+    apply matching_entry_implies_sign in m.
+    apply matching_entry_implies_sign in m0.
+    destruct e0.
+    unfold matching_entries; simpl.
+
+    eapply matching_entry_sign_trans;[|eauto].
+    eapply matching_entry_sign_sym;auto.
+Qed.
+
+Lemma find_entry_some_decomp {o} :
+  forall (lib : @library o) abs bs e,
+    find_entry lib abs bs = Some e
+    <=> {lib1 : library
+         & {lib2 : library
+         & {oa : opabs
+         & {vars : list sovar_sig
+         & {rhs : SOTerm
+         & {correct : correct_abs oa vars rhs
+         & lib = lib1 ++ e :: lib2
+         # e = lib_abs oa vars rhs correct
+         # matching_entry abs oa vars bs
+         # find_entry lib1 abs bs = None }}}}}}.
+Proof.
+  induction lib; introv; split; introv h; simpl in *; ginv.
+
+  - exrepnd.
+    destruct lib1; ginv.
+
+  - destruct a.
+    boolvar; ginv.
+
+    + exists ([] : @library o) lib opabs vars rhs correct; simpl.
+      dands; auto.
+
+    + apply IHlib in h; exrepnd; subst; clear IHlib.
+      exists (lib_abs opabs vars rhs correct :: lib1) lib2 oa vars0 rhs0 correct0.
+      dands; auto.
+      simpl; boolvar; auto.
+      apply not_matching_entry_iff in n; tcsp.
+
+  - exrepnd; subst.
+    destruct a.
+    destruct lib1; simpl in *; ginv.
+
+    + inversion h0; subst; clear h0.
+      pose proof (correct_abs_proof_irrelevance _ _ _ correct correct0) as xx; subst; auto.
+      boolvar; auto.
+      apply not_matching_entry_iff in n; tcsp.
+
+    + boolvar; ginv.
+      apply IHlib.
+      exists lib1 lib2 oa vars rhs correct; dands; auto.
+Qed.
+
+Lemma implies_entry_in_library_app_right {o} :
+  forall (lib1 lib2 : @library o) e,
+    entry_in_library e lib2
+    -> (forall e', LIn e' lib1 -> ~ matching_entries e e')
+    -> entry_in_library e (lib1 ++ lib2).
+Proof.
+  induction lib1; introv h q; simpl in *; auto.
+  right; dands; auto.
+Qed.
+
+Lemma matching_entry_trans_right {o} :
+  forall abs1 abs2 abs3 vars1 vars2 (bs : list (@BTerm o)),
+    matching_entry abs1 abs2 vars1 bs
+    -> matching_entry abs2 abs3 vars2 bs
+    -> matching_entry abs1 abs3 vars2 bs.
+Proof.
+  introv m1 m2; unfold matching_entry in *; repnd; dands; tcsp;
+    try (complete (allrw; auto)).
+  eapply matching_parameters_trans; eauto.
+Qed.
+
+Lemma matching_entry_sym {o} :
+  forall abs1 abs2 vars (bs : list (@BTerm o)),
+    matching_entry abs1 abs2 vars bs
+    -> matching_entry abs2 abs1 vars bs.
+Proof.
+  introv m; unfold matching_entry in *; repnd; dands; tcsp;
+    try (complete (allrw; auto)).
+  apply matching_parameters_sym; auto.
+Qed.
+
+Lemma matching_entry_preserves_find_entry {o} :
+  forall (lib : @library o) abs1 abs2 vars bs,
+    matching_entry abs1 abs2 vars bs
+    -> find_entry lib abs1 bs = find_entry lib abs2 bs.
+Proof.
+  induction lib; introv m; simpl in *; auto.
+  destruct a.
+  boolvar; auto.
+  - apply not_matching_entry_iff in n.
+    apply matching_entry_sym in m.
+    eapply matching_entry_trans_right in m0;[|exact m]; tcsp.
+  - apply not_matching_entry_iff in n.
+    eapply matching_entry_trans_right in m0;[|exact m]; tcsp.
+  - eapply IHlib; eauto.
+Qed.
+
+Lemma matching_entry_sign_implies_matching_entry {o} :
+  forall (abs1 abs2 : opabs) (vars : list sovar_sig) (bs : list (@BTerm o)),
+    matching_bterms vars bs
+    -> matching_entry_sign abs1 abs2
+    -> matching_entry abs1 abs2 vars bs.
+Proof.
+  introv h m; unfold matching_entry_sign in m; unfold matching_entry.
+  repnd; dands; auto.
+Qed.
+
+Lemma matching_entry_implies_matching_bterms {o} :
+  forall (abs1 abs2 : opabs) (vars : list sovar_sig) (bs : list (@BTerm o)),
+    matching_entry abs1 abs2 vars bs
+    -> matching_bterms vars bs.
+Proof.
+  introv m; unfold matching_entry in m; tcsp.
+Qed.
+
+Lemma correct_abs_implies_matching_sign {o} :
+  forall abs vars (t : @SOTerm o),
+    correct_abs abs vars t
+    -> matching_sign vars (opabs_sign abs).
+Proof.
+  introv cor.
+  unfold correct_abs in cor; tcsp.
+Qed.
+
+Lemma matching_entry_sign_implies_eq_opabs_signs :
+  forall abs1 abs2,
+    matching_entry_sign abs1 abs2
+    -> opabs_sign abs1 = opabs_sign abs2.
+Proof.
+  introv m; unfold matching_entry_sign in m; tcsp.
+Qed.
+
+Lemma find_entry_none_implies {o} :
+  forall (lib : @library o) abs bs e vars rhs correct,
+    matching_sign vars (opabs_sign abs)
+    -> matching_sign vars (map num_bvars bs)
+    -> find_entry lib abs bs = None
+    -> LIn e lib
+    -> ~ matching_entries (lib_abs abs vars rhs correct) e.
+Proof.
+  induction lib; introv ms1 ms2 fe i; simpl in *; tcsp.
+  destruct a; repndors; subst; boolvar; tcsp.
+
+  - unfold matching_entries; simpl; intro h.
+    apply not_matching_entry_iff in n.
+    destruct n.
+    apply matching_entry_sign_implies_matching_entry; auto.
+    apply matching_bterms_as_matching_sign.
+    apply correct_abs_implies_matching_sign in correct0.
+    unfold matching_sign in *.
+
+    apply matching_entry_sign_implies_eq_opabs_signs in h.
+    rewrite correct0.
+    rewrite <- h.
+    rewrite <- ms1; rewrite <- ms2; auto.
+
+  - eapply IHlib; eauto.
+Qed.
+
+Lemma entry_in_libray_implies_find_entry_some {o} :
+  forall lib abs oa vars (t : @SOTerm o) bs correct,
+    matching_entry abs oa vars bs
+    -> entry_in_library (lib_abs oa vars t correct) lib
+    -> find_entry lib abs bs = Some (lib_abs oa vars t correct).
+Proof.
+  induction lib; introv m i; simpl in *; tcsp.
+  destruct a; simpl in *.
+  repndors; repnd.
+
+  - inversion i; subst; clear i.
+    pose proof (correct_abs_proof_irrelevance _ _ _ correct correct0) as xx; subst; auto.
+    boolvar; auto.
+    apply not_matching_entry_iff in n; tcsp.
+
+  - unfold matching_entries in i0; simpl in i0.
+    boolvar; ginv.
+
+    + destruct i0.
+      eapply matching_entry_implies_sign.
+      eapply matching_entry_trans_right;[|exact m0].
+      apply matching_entry_sym;eauto.
+
+    + apply IHlib; auto.
+Qed.
+
+Lemma lib_extends_preserves_find_entry {o} :
+  forall (lib1 lib2 : @library o) abs bs (e : library_entry),
+    lib_extends lib2 lib1
+    -> find_entry lib1 abs bs = Some e
+    -> find_entry lib2 abs bs = Some e.
+Proof.
+  introv ext fe.
+  apply find_entry_some_decomp in fe; exrepnd; subst.
+
+  pose proof (ext (lib_abs oa vars rhs correct)) as h.
+  simpl in h; autodimp h hyp.
+
+  { apply implies_entry_in_library_app_right;[simpl; tcsp|].
+    pose proof (matching_entry_preserves_find_entry lib0 abs oa vars bs) as q.
+    autodimp q hyp.
+    rewrite q in fe1; clear q.
+    applydup @matching_entry_implies_matching_bterms in fe3.
+    dup correct as ms.
+    apply correct_abs_implies_matching_sign in ms.
+    rw @matching_bterms_as_matching_sign in fe0.
+    introv i; eapply find_entry_none_implies; eauto. }
+
+  apply entry_in_libray_implies_find_entry_some; auto.
+Qed.
+
+Lemma compute_step_preserves_lib_extends {o} :
+  forall (lib1 lib2 : library)
+         (ext  : lib_extends lib2 lib1) (* lib2 extends lib1 *)
+         (a b  : @NTerm o)
+         (comp : compute_step lib1 a = csuccess b),
+    compute_step lib2 a = csuccess b.
+Proof.
+  nterm_ind1s a as [v|f ind|op bs ind] Case; introv comp.
+
+  - Case "vterm".
+    csunf comp; allsimpl; ginv.
+
+  - Case "sterm".
+    csunf comp; allsimpl; ginv.
+
+  - Case "oterm".
+    dopid op as [can|ncan|exc|abs] SCase.
+
+    + SCase "Can".
+      csunf comp; allsimpl; ginv.
+
+    + SCase "NCan".
+      destruct bs as [|b1 bs]; try (complete (allsimpl; ginv)).
+      destruct b1 as [l t]; try (complete (allsimpl; ginv)).
+      destruct l; try (complete (allsimpl; ginv)).
+
+      { destruct t as [x|f|op bts]; try (complete (allsimpl; ginv));[|].
+
+        - csunf comp; allsimpl.
+          dopid_noncan ncan SSCase; allsimpl; ginv.
+
+          SSCase "NEApply".
+
+          apply compute_step_eapply_success in comp; exrepnd; subst.
+          repndors; exrepnd; allsimpl; subst.
+
+          + apply compute_step_eapply2_success in comp1; repnd; subst.
+            repndors; exrepnd; subst; ginv.
+            csunf; simpl.
+            dcwf h; simpl.
+            boolvar; try omega.
+            rewrite Znat.Nat2Z.id; auto.
+
+          + csunf; simpl.
+            apply isexc_implies2 in comp0; exrepnd; subst.
+            dcwf h; simpl; auto.
+
+          + fold_terms.
+            rewrite compute_step_eapply_iscan_isnoncan_like; auto.
+            pose proof (ind arg2 arg2 []) as h; clear ind.
+            repeat (autodimp h hyp); eauto 3 with slow.
+            apply h in comp1; clear h.
+            rewrite comp1; auto.
+
+        - dopid op as [can2|ncan2|exc2|abs2] SSCase.
+
+          + SSCase "Can".
+            dopid_noncan ncan SSSCase.
+
+            {
+              SSSCase "NApply".
+
+              csunf comp; allsimpl.
+              apply compute_step_apply_success in comp.
+              repndors; exrepnd; subst; auto.
+            }
+
+            {
+              SSSCase "NEApply".
+
+              csunf comp; allsimpl.
+              apply compute_step_eapply_success in comp.
+              repndors; exrepnd; subst; auto.
+              repndors; exrepnd; subst; allsimpl; auto.
+
+              - apply compute_step_eapply2_success in comp1; repnd; subst.
+                repndors; exrepnd; subst; auto; ginv.
+
+                + unfold mk_lam in *; ginv.
+                  csunf; simpl.
+                  dcwf h; simpl.
+                  apply iscan_implies in comp0; repndors; exrepnd; subst; simpl; auto.
+
+                + unfold mk_nseq in *; allsimpl; ginv.
+                  csunf; simpl.
+                  dcwf h; simpl.
+                  boolvar; simpl; auto; try omega.
+                  rewrite Znat.Nat2Z.id; auto.
+
+              - fold_terms; rewrite compute_step_eapply_iscan_isexc; auto.
+
+              - fold_terms; rewrite compute_step_eapply_iscan_isnoncan_like; auto.
+
+                pose proof (ind arg2 arg2 []) as q; clear ind.
+                repeat (autodimp q hyp); eauto 2 with slow.
+                apply q in comp1; clear q.
+                rewrite comp1; auto.
+            }
+
+            {
+              SSSCase "NFix".
+
+              csunf comp; allsimpl.
+              apply compute_step_fix_success in comp.
+              repndors; exrepnd; subst; auto.
+            }
+
+            {
+              SSSCase "NSpread".
+
+              csunf comp; allsimpl.
+              apply compute_step_spread_success in comp.
+              repndors; exrepnd; subst; auto.
+            }
+
+            {
+              SSSCase "NDsup".
+
+              csunf comp; allsimpl.
+              apply compute_step_dsup_success in comp.
+              repndors; exrepnd; subst; auto.
+            }
+
+            {
+              SSSCase "NDecide".
+
+              csunf comp; allsimpl.
+              apply compute_step_decide_success in comp.
+              repndors; exrepnd; subst; auto.
+              repndors; exrepnd; subst; auto.
+            }
+
+            {
+              SSSCase "NCbv".
+
+              csunf comp; allsimpl.
+              apply compute_step_cbv_success in comp.
+              repndors; exrepnd; subst; auto.
+            }
+
+            {
+              SSSCase "NSleep".
+
+              csunf comp; allsimpl.
+              apply compute_step_sleep_success in comp.
+              repndors; exrepnd; subst; auto.
+            }
+
+            {
+              SSSCase "NTUni".
+
+              csunf comp; allsimpl.
+              apply compute_step_tuni_success in comp.
+              repndors; exrepnd; subst; auto.
+              csunf; simpl.
+              unfold compute_step_tuni; simpl.
+              boolvar; try omega.
+              rewrite Znat.Nat2Z.id; auto.
+            }
+
+            {
+              SSSCase "NMinus".
+
+              csunf comp; allsimpl.
+              apply compute_step_minus_success in comp.
+              repndors; exrepnd; subst; auto.
+            }
+
+            {
+              SSSCase "NFresh".
+
+              csunf comp; allsimpl; ginv.
+            }
+
+            {
+              SSSCase "NTryCatch".
+
+              csunf comp; allsimpl.
+              apply compute_step_try_success in comp.
+              repndors; exrepnd; subst; auto.
+            }
+
+            {
+              SSSCase "NParallel".
+
+              csunf comp; allsimpl.
+              apply compute_step_parallel_success in comp.
+              repndors; exrepnd; subst; auto.
+            }
+
+            {
+              SSSCase "NCompOp".
+
+              apply compute_step_ncompop_can1_success in comp; repnd.
+              repndors; exrepnd; allsimpl; subst; tcsp.
+
+              - csunf; simpl.
+                dcwf h.
+
+              - rewrite compute_step_ncompop_ncanlike2; auto.
+                dcwf h.
+                pose proof (ind t t []) as q; clear ind.
+                repeat (autodimp q hyp); eauto 2 with slow.
+                apply q in comp4; clear q.
+                rewrite comp4; auto.
+
+              - csunf; simpl.
+                apply isexc_implies2 in comp1; exrepnd; subst.
+                dcwf h; simpl; auto.
+            }
+
+            {
+              SSSCase "NArithOp".
+
+              apply compute_step_narithop_can1_success in comp; repnd.
+              repndors; exrepnd; allsimpl; subst; tcsp.
+
+              - csunf; simpl.
+                dcwf h.
+
+              - rewrite compute_step_narithop_ncanlike2; auto.
+                dcwf h.
+                pose proof (ind t t []) as q; clear ind.
+                repeat (autodimp q hyp); eauto 2 with slow.
+                apply q in comp4; clear q.
+                rewrite comp4; auto.
+
+              - csunf; simpl.
+                apply isexc_implies2 in comp1; exrepnd; subst.
+                dcwf h; simpl; auto.
+            }
+
+            {
+              SSSCase "NCanTest".
+
+              csunf comp; allsimpl.
+              apply compute_step_can_test_success in comp.
+              repndors; exrepnd; subst; auto.
+            }
+
+          + SSCase "NCan".
+
+            csunf comp; allsimpl.
+            remember (compute_step lib1 (oterm (NCan ncan2) bts)) as c.
+            destruct c; allsimpl; ginv.
+            symmetry in Heqc.
+
+            pose proof (ind (oterm (NCan ncan2) bts) (oterm (NCan ncan2) bts) []) as q; clear ind.
+            repeat (autodimp q hyp); eauto 2 with slow.
+            apply q in Heqc; clear q.
+            csunf; simpl.
+            rewrite Heqc; auto.
+
+          + SSCase "Exc".
+
+            csunf comp; allsimpl.
+            apply compute_step_catch_success in comp.
+            repndors; exrepnd; subst; allsimpl; ginv.
+
+            * csunf; simpl; auto.
+
+            * csunf; simpl; auto.
+              rewrite compute_step_catch_if_diff; auto.
+
+          + SSCase "Abs".
+
+            csunf comp; allsimpl.
+            remember (compute_step lib1 (oterm (Abs abs2) bts)) as c.
+            destruct c; allsimpl; ginv.
+            symmetry in Heqc.
+
+            pose proof (ind (oterm (Abs abs2) bts) (oterm (Abs abs2) bts) []) as q; clear ind.
+            repeat (autodimp q hyp); eauto 2 with slow.
+            apply q in Heqc; clear q.
+            csunf; simpl.
+            rewrite Heqc; auto.
+      }
+
+      {
+        csunf comp; allsimpl.
+        apply compute_step_fresh_success in comp; exrepnd; subst.
+        repndors; exrepnd; subst; ginv.
+
+        - csunf; simpl; boolvar; auto.
+
+        - rewrite compute_step_fresh_if_isvalue_like2; auto.
+
+        - fold (mk_fresh n t).
+          rewrite compute_step_fresh_if_isnoncan_like; auto.
+
+          pose proof (ind t (subst t n (mk_utoken (get_fresh_atom t))) [n]) as q; clear ind.
+          repeat (autodimp q hyp); eauto 2 with slow.
+          { rewrite simple_osize_subst; eauto 2 with slow. }
+          apply q in comp2; clear q.
+          remember (get_fresh_atom t) as a; simpl.
+          rewrite comp2; simpl; auto.
+      }
+
+    + SCase "Exc".
+
+      csunf comp; allsimpl; ginv.
+
+    + SCase "Abs".
+
+      csunf comp; allsimpl.
+      apply compute_step_lib_success in comp.
+      exrepnd; subst.
+
+      csunf; simpl.
+
+      apply (found_entry_implies_compute_step_lib_success _ _ _ _ _ _ correct).
+      eapply lib_extends_preserves_find_entry; eauto.
+Qed.
+
+Lemma reduces_to_preserves_lib_extends {o} :
+  forall (lib1 lib2 : library)
+         (ext  : lib_extends lib2 lib1) (* lib2 extends lib1 *)
+         (a b  : @NTerm o)
+         (comp : reduces_to lib1 a b),
+    reduces_to lib2 a b.
+Proof.
+  introv ext r.
+  unfold reduces_to in *; exrepnd.
+  exists k.
+  revert dependent a.
+  induction k; introv r.
+
+  - allrw @reduces_in_atmost_k_steps_0; auto.
+
+  - allrw @reduces_in_atmost_k_steps_S; exrepnd.
+    exists u; dands; auto.
+    eapply compute_step_preserves_lib_extends; eauto.
+Qed.
